proof/theories/Bytecode.v
@@ -61,6 +61,7 @@ Inductive instr : Type :=
 | ICmp         (op : cmpop) (src : reg) (v : data)
 | IRange       (op : cmpop) (src : reg) (lo hi : data)   (* range eq/neq *)
 | IBitwise     (dst src : reg) (mask xor : data)         (* dst = (src & mask) ^ xor *)
+| IBitwiseOr   (dst src1 src2 : reg)                     (* dst = src1 | src2 *)
 | IBitShift    (dst src : reg) (shl : bool) (amt : nat) (* dst = src >>/<< amt *)
 | IByteorder   (dst src : reg) (hton : bool) (size len : nat)
 | IJhash       (dst src : reg) (len seed modulus offset : nat)
